Hashmap/Henrik.lean
@@ -12,15 +12,15 @@ variable {α : Type u} [BEq α] [Hashable α] [LawfulHashable α]
 inductive Inv1 : Nat → HashMap α Nat → Prop where
 | empty : Inv1 0 {}
 | insert {n : Nat} {map : HashMap α Nat} {x : α}
-    (hinv : Inv1 n map) (hfind : map.find? x = none) : Inv1 (n + 1) (map.insert x n)
+    (hinv : Inv1 n map) (hfind : map[x]? = none) : Inv1 (n + 1) (map.insert x n)
 
 theorem Inv1.property₂ [EquivBEq α] {n m : Nat} (map : HashMap α Nat) (x : α) (hinv : Inv1 n map) :
-    map.find? x = some m → m < n := by
+    map[x]? = some m → m < n := by
   induction hinv
   · simp
   · next k m' y ih₁ ih₂ ih₃ =>
     skip
-    rw [HashMap.find?_insert]
+    rw [HashMap.getElem?_insert]
     cases y == x
     · rw [cond_false]
       intro h
@@ -30,13 +30,13 @@ theorem Inv1.property₂ [EquivBEq α] {n m : Nat} (map : HashMap α Nat) (x : �
       exact Nat.lt_succ_self _
 
 theorem Inv1.property' [EquivBEq α] {n m : Nat} (x y : α) (map : HashMap α Nat) (hinv : Inv1 n map)
-    (hfound1 : map.find? x = some m) (hfound2 : map.find? y = some m) : x == y := by
+    (hfound1 : map[x]? = some m) (hfound2 : map[y]? = some m) : x == y := by
   induction hinv
   · simp at hfound1
   · next k m' x' ih₁ _ ih₃ =>
     skip
-    rw [HashMap.find?_insert] at hfound1
-    rw [HashMap.find?_insert] at hfound2
+    rw [HashMap.getElem?_insert] at hfound1
+    rw [HashMap.getElem?_insert] at hfound2
     cases hx : x' == x
     · rw [hx, cond_false] at hfound1
       cases hy : x' == y
@@ -55,5 +55,5 @@ theorem Inv1.property' [EquivBEq α] {n m : Nat} (x y : α) (map : HashMap α Na
       · exact (BEq.trans (BEq.symm hx) hy)
 
 theorem Inv1.property [LawfulBEq α] {n m : Nat} (x y : α) (map : HashMap α Nat) (hinv : Inv1 n map)
-    (hfound1 : map.find? x = some m) (hfound2 : map.find? y = some m) : x = y :=
+    (hfound1 : map[x]? = some m) (hfound2 : map[y]? = some m) : x = y :=
   eq_of_beq (Inv1.property' x y map hinv hfound1 hfound2)
